CheckPartrec.lean
@@ -1,0 +1,2 @@
+import Mathlib.Computability.Partrec
+#check Partrec
